theories/modules/ModTr.v
@@ -1,25 +1,24 @@
-Require Import Common.
-Require Import FSpec LMod.
-
-Set Implicit Arguments.
+Require Import Common FSpec LMod.
 
 Module ModTr. Section MID.
   Context `{Σ : GRA}.
 
   (* Consider moving into Any lib. *)
-  (* Any.encode & Any.decode *)
-  (* local states : [(k0, st0); (k1, st1); ... ] *)
-  Fixpoint _alist_encode (st_list : alist key Any.t) : Any.t :=
+  Fixpoint _state_encode (st_list : list (key * option Any.t)) : Any.t :=
     match st_list with
     | [] => tt↑
-    | (k,v) ::tl =>
-      Any.pair (Any.pair k↑ v) (_alist_encode tl)
+    | (k, Some v) :: tl => Any.pair (Any.pair k↑ v) (_state_encode tl)
+    | (k, None) :: tl => _state_encode tl
     end.
 
-  Definition alist_encode st_list :=
-    Any.pair (List.length st_list)↑ (_alist_encode st_list).
+  (* Definition alist_encode st_list :=
+    Any.pair (List.length st_list)↑ (_alist_encode st_list). *)
 
-  Fixpoint _alist_decode (data : Any.t) (n : nat) : alist key Any.t :=
+  (* Encode states into Any.t for state interpretation *)
+  Definition state_encode (st : gmap key (option Any.t)) : Any.t :=
+    Any.pair (size st)↑ (_state_encode (map_to_list st)).
+
+  Fixpoint _state_decode (data : Any.t) (n : nat) : gmap key (option Any.t) :=
     match n with
     | S n' =>
         match Any.split data with
@@ -27,63 +26,61 @@ Module ModTr. Section MID.
             match Any.split kv with
             | Some (ka, v) =>
                 match ka↓ with
-                | Some k => (k,v) :: _alist_decode data' n'
-                | None => []
+                | Some k => <[k := Some v]> (_state_decode data' n')
+                | None => ∅
                 end
-            | None => []
+            | None => ∅
             end
-        | None => []
+        | None => ∅
         end
-    | 0 => []
+    | 0 => ∅
     end.
 
-  Definition alist_decode st :=
+  Definition state_decode (st : Any.t) : gmap key (option Any.t) :=
     match Any.split st with
     | Some (na, data) =>
         match na↓ with
-        | Some n => _alist_decode data n
-        | None => []
+        | Some n => _state_decode data n
+        | None => ∅
         end
-    | None => []
+    | None => ∅
     end.
 
-  Lemma alist_encode_decode st :
-    alist_decode (alist_encode st) = st.
+  Lemma state_encode_decode (st : gmap key (option Any.t)) :
+    map_Forall (λ _ v, is_Some v) st →
+    state_decode (state_encode st) = st.
   Proof using.
-    unfold alist_encode, alist_decode.
-    rewrite Any.pair_split; rewrite Any.upcast_downcast; eauto.
-    induction st; s; eauto.
-    destruct a.
-    s; rewrite !Any.pair_split; rewrite Any.upcast_downcast; eauto.
-    rewrite IHst. eauto.
+    rewrite /state_decode /state_encode Any.pair_split Any.upcast_downcast.
+    rewrite -{3 4}(list_to_map_to_list st) map_Forall_to_list map_size_list_to_map; cycle 1.
+    { apply NoDup_fst_map_to_list. }
+    generalize (map_to_list st) as st'; clear st.
+    induction 1 as [|[k [v|]] tl Hs Hwf]; ss; [|inv Hs].
+    rewrite ?Any.pair_split Any.upcast_downcast IHHwf //.
   Qed.
 
   Definition put_res (mr : Σ) : itree lmodE unit :=
-    st <- trigger sGet;; '(mp, _) :_ <- (Any.split st)?;;
+    st <- trigger sGet;;
+    '(mp, _) :_ <- (Any.split st)?;;
     trigger (sPut (Any.pair mp mr↑)).
 
-  Definition get_res {R} (k: Σ → itree lmodE R) : itreeV lmodE R :=
+  Definition get_res {R} (k : Σ → itree lmodE R) : itreeV lmodE R :=
     inr (existT Any.t (subevent _ sGet, λ st,
       '(_, mr) : _ <- (Any.split st)?;;
       r <- mr↓?;; k r)).
 
-  Definition mput_kv (k: key) (v: Any.t) : itreeV lmodE unit :=
+  Definition mput_kv (k : key) (v : Any.t) : itreeV lmodE unit :=
     inr (existT Any.t (subevent _ sGet, λ st,
-      or_else (
+      default (Ret tt) (
         do '(mp, mr) <- Any.split st;
-        Some (trigger (sPut (Any.pair (alist_encode (alist_upd k v (alist_decode mp))) mr)))
-      )
-      ( Ret tt )))
-  .
+        Some (trigger (sPut (Any.pair (state_encode (<[k := Some v]> (state_decode mp))) mr)))
+      ))).
 
-  Definition mget_kv (k: key) : itreeV lmodE Any.t :=
+  Definition mget_kv (k : key) : itreeV lmodE Any.t :=
     inr (existT Any.t (subevent _ sGet, λ st,
-      or_else (
+      default (Ret tt↑) (
         do '(mp, _) <- Any.split st;
-        Some (Ret (or_else (alist_find k (alist_decode mp)) tt↑))
-      )
-      ( Ret tt↑ )))
-  .
+        Some (Ret (default tt↑ (mjoin (state_decode mp !! k))))
+      ))).
 
   (* mid to tgt code *)
   Definition handle_pgE : pgE ~> itreeV lmodE :=
@@ -121,98 +118,100 @@ Module ModTr. Section MID.
   Definition handle_crisE : crisE ~> itreeV lmodE :=
     λ T e,
       match e with
-      | inl1 ag => handle_agE ag
+      | inl1 ag => handle_agE _ ag
       | inr1 (inl1 c) => inr (existT T (subevent _ c, λ r, Ret r))
-      | inr1 (inr1 (inl1 pg)) => handle_pgE pg
+      | inr1 (inr1 (inl1 pg)) => handle_pgE _ pg
       | inr1 (inr1 (inr1 c)) => inr (existT T (subevent _ c, λ r, Ret r))
       end.
 
   Definition trans : itree crisE ~> itree lmodE :=
     interpV handle_crisE.
 
-  Definition trans_ktree (f : Any.t → itree crisE Any.t) : Any.t → itree lmodE Any.t :=
-    λ x, trans (f x).
+  Definition trans_fnsem (f : Any.t → itree crisE Any.t) : Any.t → itree lmodE Any.t :=
+    λ x, trans _ (f x).
 End MID. End ModTr.
+Arguments ModTr.trans {Σ T}.
 
 Module Red. Section RED.
+  Import ModTr.
   (* itree reduction lemmas *)
   Context `{Σ : GRA}.
 
-  Lemma bind (R S : Type) (s : itree crisE R) (k : R → itree crisE S) :
-    ModTr.trans (s >>= k) = st <- ModTr.trans s;; ModTr.trans (k st).
-  Proof using. rewrite /ModTr.trans interpV_bind //. Qed.
+  Lemma bind {R S : Type} (s : itree crisE R) (k : R → itree crisE S) :
+    trans (s >>= k) = st <- trans s;; trans (k st).
+  Proof using. rewrite /trans interpV_bind //. Qed.
 
-  Lemma tau (R : Type) (t : itree _ R) :
-    ModTr.trans (tau;; t) = tau;; (ModTr.trans t).
-  Proof using. rewrite /ModTr.trans interpV_tau //. Qed.
+  Lemma tau {R : Type} (t : itree _ R) :
+    trans (tau;; t) = tau;; (trans t).
+  Proof using. rewrite /trans interpV_tau //. Qed.
 
-  Lemma ret (R : Type) (t : R) :
-    ModTr.trans (Ret t) = Ret t.
-  Proof using. rewrite /ModTr.trans interpV_ret //. Qed.
+  Lemma ret {R : Type} (t : R) :
+    trans (Ret t) = Ret t.
+  Proof using. rewrite /trans interpV_ret //. Qed.
 
-  Lemma call (R : Type) (c : callE R) :
-    ModTr.trans (trigger c) = trigger c.
-  Proof using. rewrite /ModTr.trans interpV_trigger. s. ired. et. Qed.
+  Lemma call {R : Type} (c : callE R) :
+    trans (trigger c) = trigger c.
+  Proof using. rewrite /trans interpV_trigger /=; grind. Qed.
 
   Lemma spawn fn arg :
-    ModTr.trans (trigger (Spawn fn arg)) = trigger (Spawn fn arg).
-  Proof using. rewrite /ModTr.trans interpV_trigger. s. ired. et. Qed.
+    trans (trigger (Spawn fn arg)) = trigger (Spawn fn arg).
+  Proof using. rewrite /trans interpV_trigger /=; grind. Qed.
 
   Lemma yield tid :
-    ModTr.trans (trigger (Yield tid)) = trigger (Yield tid).
-  Proof using. rewrite /ModTr.trans interpV_trigger. s. ired. et. Qed.
+    trans (trigger (Yield tid)) = trigger (Yield tid).
+  Proof using. rewrite /trans interpV_trigger /=; grind. Qed.
 
-  Lemma pg (R : Type) (i : pgE R) :
-    ModTr.trans (trigger i) = itreeV_itree (ModTr.handle_pgE i).
-  Proof using. rewrite /ModTr.trans interpV_trigger //. Qed.
+  Lemma pg {R : Type} (i : pgE R) :
+    trans (trigger i) = itreeV_itree (handle_pgE _ i).
+  Proof using. rewrite /trans interpV_trigger //. Qed.
 
-  Lemma core (R : Type) (i : coreE R) :
-    ModTr.trans (trigger i) = trigger i.
-  Proof using. rewrite /ModTr.trans interpV_trigger. s. ired. et. Qed.
+  Lemma core {R : Type} (i : coreE R) :
+    trans (trigger i) = trigger i.
+  Proof using. rewrite /trans interpV_trigger /=; grind. Qed.
 
-  Lemma triggerUB (R : Type) :
-    ModTr.trans (triggerUB) = triggerUB (A:=R).
+  Lemma triggerUB {R : Type} :
+    trans (triggerUB) = triggerUB (A:=R).
   Proof using.
-    rewrite /ModTr.trans /triggerUB interpV_bind interpV_trigger; grind.
+    rewrite /trans /triggerUB interpV_bind interpV_trigger; grind.
   Qed.
 
-  Lemma triggerNB (R : Type) :
-    ModTr.trans (triggerNB) = triggerNB (A:=R).
+  Lemma triggerNB {R : Type} :
+    trans (triggerNB) = triggerNB (A:=R).
   Proof using.
-    rewrite /ModTr.trans /triggerNB interpV_bind interpV_trigger; grind.
+    rewrite /trans /triggerNB interpV_bind interpV_trigger; grind.
   Qed.
 
-  Lemma unwrapU (R : Type) (i : option R) :
-    ModTr.trans (@unwrapU crisE _ _ i) = unwrapU i.
+  Lemma unwrapU {R : Type} (i : option R) :
+    trans (@unwrapU crisE _ _ i) = unwrapU i.
   Proof using.
-    rewrite /ModTr.trans /unwrapU; des_ifs; s; try rewrite interpV_ret; eauto using triggerUB.
+    rewrite /trans /unwrapU; des_ifs; s; try rewrite interpV_ret; eauto using triggerUB.
   Qed.
 
-  Lemma unwrapN (R : Type) (i : option R) :
-    ModTr.trans (@unwrapN crisE _ _ i) = unwrapN i.
+  Lemma unwrapN {R : Type} (i : option R) :
+    trans (@unwrapN crisE _ _ i) = unwrapN i.
   Proof using.
-    rewrite /ModTr.trans /unwrapN; des_ifs; s; try rewrite interpV_ret; eauto using triggerNB.
+    rewrite /trans /unwrapN; des_ifs; s; try rewrite interpV_ret; eauto using triggerNB.
   Qed.
 
   Lemma Assume P :
-    ModTr.trans (trigger (Assume P)) = itreeV_itree (ModTr.handle_Assume P).
-  Proof using. rewrite /ModTr.trans interpV_trigger //. Qed.
+    trans (trigger (Assume P)) = itreeV_itree (handle_Assume P).
+  Proof using. rewrite /trans interpV_trigger //. Qed.
 
-  Lemma AssumeRes P :
-    ModTr.trans (trigger (AssumeRes P)) = itreeV_itree (ModTr.handle_AssumeRes P).
-  Proof using. rewrite /ModTr.trans interpV_trigger //. Qed.
+  Lemma AssumeRes r :
+    trans (trigger (AssumeRes r)) = itreeV_itree (handle_AssumeRes r).
+  Proof using. rewrite /trans interpV_trigger //. Qed.
   
   Lemma Guarantee P :
-    ModTr.trans (trigger (Guarantee P)) = itreeV_itree (ModTr.handle_Guarantee P).
-  Proof using. rewrite /ModTr.trans interpV_trigger //. Qed.
+    trans (trigger (Guarantee P)) = itreeV_itree (handle_Guarantee P).
+  Proof using. rewrite /trans interpV_trigger //. Qed.
 
-  Lemma ext R (itr0 itr1 : itree _ R) (EQ : itr0 = itr1) :
-    ModTr.trans itr0 = ModTr.trans itr1.
+  Lemma ext {R : Type} (itr0 itr1 : itree _ R) (EQ : itr0 = itr1) :
+    trans itr0 = trans itr1.
   Proof using. subst; et. Qed.
 
   (* TODO : Same lemmas for other interps ( not defined yet. ) *)
 
-  Global Program Instance rdb : red_database (mk_box (@ModTr.trans)) :=
+  (* Global Program Instance rdb : red_database (mk_box (@trans)) :=
     mk_rdb
       0
       (mk_box bind)
@@ -229,5 +228,5 @@ Module Red. Section RED.
       (mk_box unwrapN)
       (mk_box Assume)
       (mk_box Guarantee)
-      (mk_box ext).
+      (mk_box ext). *)
 End RED. End Red.
